Engine: rename PikeVMSeen into PikeVM, PikeTreeSeen into PikeTree and PikeSeenEquiv into PikeEquiv

Engine/PikeEquiv.v
@@ -1,1 +1,958 @@
 (* Relating the PikeVM smallstep semantics to the Pike Tree smallstep semantics *)
+
+Require Import List Lia.
+Import ListNotations.
+
+From Linden Require Import Regex Chars Groups.
+From Linden Require Import Tree Semantics BooleanSemantics.
+From Linden Require Import NFA PikeTree PikeVM.
+From Linden Require Import PikeSubset.
+From Linden Require Import TreeRep.
+From Warblre Require Import Base RegExpRecord.
+
+
+Section PikeEquiv.
+  Context (rer: RegExpRecord).
+
+(** * Simulation Invariant  *)
+
+(* a tree and a thread are equivalent when they are about to execute the same thing *)
+(* this means when the tree represents a given list of actions, *)
+(* the thread is at a pc that will execute the nfa of that same list of actions *)
+Inductive tree_thread (code:code) (inp:input) : (tree * group_map) -> thread -> Prop :=
+| tt_eq:
+  forall tree gm pc b actions
+    (TREE: bool_tree rer actions inp b tree)
+    (CONT: actions_rep actions code pc)
+    (SUBSET: pike_actions actions),
+    tree_thread code inp (tree, gm) (pc, gm, b)
+| tt_reset:
+  forall tree gm pc b gidl
+    (TT: tree_thread code inp (tree,GroupMap.reset gidl gm) (pc+1,GroupMap.reset gidl gm,b))
+    (RESET: get_pc code pc = Some (ResetRegs gidl)),
+    tree_thread code inp (GroupAction (Reset gidl) tree,gm) (pc,gm,b)
+| tt_begin:
+  forall tree gm pc b
+    (TT: tree_thread code inp (tree,gm) (pc+1,gm,CannotExit))
+    (BEGIN: get_pc code pc = Some BeginLoop),
+    tree_thread code inp (tree,gm) (pc,gm,b).
+    
+
+(* the initial active thread and the initial active tree are related with the invariant *)
+Lemma initial_tree_thread:
+  forall r code tree inp
+    (COMPILE: compilation r = code)
+    (TREE: bool_tree rer [Areg r] inp CanExit tree)
+    (SUBSET: pike_regex r),
+    tree_thread code inp (tree, GroupMap.empty) (0, GroupMap.empty, CanExit).
+Proof.
+  intros r code tree inp COMPILE TREE SUBSET.
+  unfold compilation in COMPILE. destruct (compile r 0) as [c fresh] eqn:COMP.
+  apply compile_nfa_rep with (prev := []) in COMP as REP; auto. simpl in REP.
+  apply fresh_correct in COMP. simpl in COMP. subst.
+  subst. eapply tt_eq; eauto.
+  2: { repeat (constructor; auto). }
+  apply cons_bc with (pcmid := length c).
+  - constructor. apply nfa_rep_extend. auto.
+  - constructor. replace (length c) with (length c + 0) by auto. rewrite get_prefix. auto.
+Qed.
+
+(* lifting the equivalence predicate to lists *)
+Inductive list_tree_thread (code:code) (inp:input) : list (tree * group_map) -> list thread -> Prop :=
+| ltt_nil: list_tree_thread code inp [] []
+| ltt_cons:
+  forall treelist threadlist tree gm pc b
+    (LTT: list_tree_thread code inp treelist threadlist)
+    (TT: tree_thread code inp (tree, gm) (pc, gm, b)),
+    list_tree_thread code inp ((tree,gm)::treelist) ((pc,gm,b)::threadlist).
+
+Lemma ltt_app:
+  forall code inp tl1 tl2 vl1 vl2
+    (LTT1: list_tree_thread code inp tl1 vl1)
+    (LTT2: list_tree_thread code inp tl2 vl2),
+    list_tree_thread code inp (tl1 ++ tl2) (vl1 ++ vl2).
+Proof.
+  intros. induction LTT1; auto. simpl. econstructor; eauto.
+Qed.
+
+(** * Invariant Preservation  *)
+
+(* generate lemmas: *)
+(* For each possible kind of tree, I show that the PikeTree step over that tree corresponds *)
+(* to an equivalent step in the PikeVM. This preserves the invariant. *)
+(* These lemmas discard the stuttering steps by preventing the current pc being at a Jmp instruction *)
+
+Theorem generate_match:
+  forall tree gm inp code pc b
+    (TREESTEP: tree_bfs_step tree gm (idx inp) = StepMatch)
+    (NOSTUTTER: stutters pc code = false)
+    (TT: tree_thread code inp (tree, gm) (pc, gm, b)),
+    epsilon_step rer (pc, gm, b) code inp = EpsMatch.
+Proof.
+  intros tree gm inp code pc b TREESTEP NOSTUTTER TT.
+  unfold tree_bfs_step in TREESTEP. destruct tree; inversion TREESTEP. subst. clear TREESTEP.
+  inversion TT; subst; try no_stutter.
+  remember Match as TMATCH.
+  (* here we have to proceed by induction because there are many ways to get a Match tree *)
+  (* it could be epsilon, it could be epsilon followed by epsilon etc *)
+  induction TREE; intros; subst; try inversion HeqTMATCH.
+  - simpl. repeat invert_rep.
+    rewrite ACCEPT. auto.
+  - repeat invert_rep. pike_subset.
+  - repeat invert_rep. eapply IHTREE; eauto. pike_subset.
+    repeat (econstructor; eauto). pike_subset.
+  - repeat invert_rep.
+  - destruct greedy; inversion CHOICE.
+ Qed.
+
+
+Theorem generate_blocked:
+  forall tree gm inp code pc b nexttree
+    (TREESTEP: tree_bfs_step tree gm (idx inp) = StepBlocked nexttree)
+    (NOSTUTTER: stutters pc code = false)
+    (TT: tree_thread code inp (tree, gm) (pc, gm, b)),
+    epsilon_step rer (pc,gm,b) code inp = EpsBlocked (pc+1,gm,CanExit) /\
+      (forall nextinp, advance_input inp forward = Some nextinp -> tree_thread code nextinp (nexttree,gm) (pc+1,gm,CanExit)) /\
+      exists nextinp, advance_input inp forward = Some nextinp.
+Proof.
+  intros tree gm inp code pc b nexttree TREESTEP NOSTUTTER TT.
+  unfold tree_bfs_step in TREESTEP. destruct tree; inversion TREESTEP. subst. clear TREESTEP.
+  inversion TT; subst; try no_stutter.
+  remember (Read c nexttree) as TREAD.
+  induction TREE; intros; subst; try inversion HeqTREAD; subst.
+  - repeat invert_rep. eapply IHTREE; eauto. pike_subset.
+  - assert (CHECK: check_read rer cd inp forward = CanRead /\ advance_input inp forward = Some nextinp) by (apply can_read_correct; eauto).
+    destruct CHECK as [CHECK ADVANCE].
+    repeat invert_rep. split; try split; eauto.
+    + simpl. rewrite CONSUME. rewrite CHECK. auto.
+    + intros. rewrite ADVANCE in H. inversion H. subst.
+      eapply tt_eq; eauto.
+      2: { pike_subset. }
+      replace (pc + 1) with (S pc) by lia. eauto.
+  - repeat invert_rep. eapply IHTREE; eauto. pike_subset.
+    repeat (econstructor; eauto). pike_subset.
+  - repeat invert_rep. 
+  - destruct greedy; inversion CHOICE.
+Qed.
+
+
+Theorem generate_open:
+  forall gid tree gm inp code pc b
+    (TT: tree_thread code inp (GroupAction (Open gid) tree, gm) (pc, gm, b))
+    (NOSTUTTER: stutters pc code = false),
+    epsilon_step rer (pc, gm, b) code inp = EpsActive [(pc + 1, GroupMap.open (idx inp) gid gm, b)] /\
+      tree_thread code inp (tree,GroupMap.open (idx inp) gid gm) (pc + 1, GroupMap.open (idx inp) gid gm, b).
+Proof.
+  intros gid tree gm inp code pc b TT NOSTUTTER.
+  inversion TT; subst; try invert_rep.
+  remember (GroupAction (Open gid) tree) as TOPEN.
+  induction TREE; intros; subst; try inversion HeqTOPEN; subst.
+  - repeat invert_rep. eapply IHTREE; eauto. pike_subset.
+  - repeat invert_rep. eapply IHTREE; eauto. pike_subset.
+    repeat (econstructor; eauto). pike_subset.
+  - repeat invert_rep.
+  - destruct greedy; inversion CHOICE.
+  - repeat invert_rep. simpl. rewrite OPEN. split; auto.
+    eapply tt_eq; eauto.
+    2: { pike_subset. }
+    replace (pc+1) with (S pc) by lia. 
+    apply cons_bc with (pcmid:=end1); repeat (econstructor; eauto).
+Qed.
+
+
+
+Theorem generate_close:
+  forall gid tree gm inp code pc b
+    (TT: tree_thread code inp (GroupAction (Close gid) tree, gm) (pc, gm, b))
+    (NOSTUTTER: stutters pc code = false),
+    epsilon_step rer (pc, gm, b) code inp = EpsActive [(pc + 1, GroupMap.close (idx inp) gid gm, b)] /\
+      tree_thread code inp (tree,GroupMap.close (idx inp) gid gm) (pc + 1, GroupMap.close (idx inp) gid gm, b).
+Proof.
+  intros gid tree gm inp code pc b TT NOSTUTTER.
+  inversion TT; subst; try no_stutter.
+  remember (GroupAction (Close gid) tree) as TCLOSE.
+  induction TREE; intros; subst; try inversion HeqTCLOSE; subst.
+  - repeat invert_rep. simpl. rewrite CLOSE. split; auto.
+    econstructor; eauto. 2: pike_subset.
+    replace (pc + 1) with (S pc) by lia. auto. 
+  - repeat invert_rep. eapply IHTREE; eauto. pike_subset.
+  - repeat invert_rep. eapply IHTREE; eauto. pike_subset.
+    repeat (econstructor; eauto). pike_subset.
+  - repeat invert_rep.
+  - destruct greedy; inversion CHOICE.
+Qed.
+
+
+Theorem no_tree_reset:
+  (* A tree corresponding to some actions cannot start with ResetGroups *)
+  forall gidl tree inp actions b,
+    pike_actions actions ->
+    bool_tree rer actions inp b (GroupAction (Reset gidl) tree) -> False.
+Proof.
+  intros gidl tree inp actions b PIKE H.
+  remember (GroupAction (Reset gidl) tree) as TRESET.
+  induction H; inversion HeqTRESET; subst; auto.
+  - pike_subset.
+  - apply IHbool_tree; auto. pike_subset.
+  - pike_subset.
+  - apply IHbool_tree; auto. pike_subset.
+  - destruct greedy; inversion CHOICE.
+Qed.
+
+Corollary generate_reset:  
+  forall gidl tree inp code pc b gm
+    (TT: tree_thread code inp (GroupAction (Reset gidl) tree, gm) (pc,gm,b))
+    (NOSTUTTER: stutters pc code = false),
+    epsilon_step rer (pc,gm,b) code inp = EpsActive [(pc+1, GroupMap.reset gidl gm, b)] /\
+      tree_thread code inp (tree,GroupMap.reset gidl gm) (pc+1, GroupMap.reset gidl gm, b).
+Proof.
+  intros.
+  inversion TT; subst.
+  - exfalso. eapply no_tree_reset; eauto.
+  - simpl. rewrite RESET. split; auto.
+  - exfalso. eapply doesnt_stutter_begin; eauto.
+Qed.
+
+Theorem generate_mismatch:
+  forall gm inp code pc b
+    (TT: tree_thread code inp (Mismatch, gm) (pc, gm, b))
+    (NOSTUTTER: stutters pc code = false),
+    epsilon_step rer (pc, gm, b) code inp = EpsActive [].
+Proof.
+  intros gm inp code pc b TT NOSTUTTER.
+  inversion TT; subst; try no_stutter.
+  remember (Mismatch) as TMIS.
+  induction TREE; intros; subst; try inversion HeqTMIS; subst.
+  - repeat invert_rep. simpl. rewrite END. auto.
+  - repeat invert_rep. eapply IHTREE; eauto. pike_subset.
+  - assert (CHECK: check_read rer cd inp forward = CannotRead) by (apply cannot_read_correct; auto).
+    repeat invert_rep. simpl. rewrite CONSUME. rewrite CHECK. auto.
+  - repeat invert_rep. eapply IHTREE; eauto. pike_subset.
+    repeat (econstructor; eauto). pike_subset.
+  - pike_subset.
+  - destruct greedy; inversion CHOICE.
+  - pike_subset.
+Qed.
+
+Theorem generate_checkpass:
+  forall tree gm inp code pc b
+    (TT: tree_thread code inp (Progress tree, gm) (pc, gm, b))
+    (NOSTUTTER: stutters pc code = false),
+    exists nextpc, epsilon_step rer (pc, gm, b) code inp = EpsActive [(nextpc,gm,CanExit)] /\
+      tree_thread code inp (tree,gm) (nextpc,gm,CanExit).
+Proof.
+  intros tree gm inp code pc b TT NOSTUTTER.
+  inversion TT; subst; try no_stutter.
+  remember (Progress tree) as TPASS.
+  induction TREE; intros; subst; try inversion HeqTPASS; subst.
+  - repeat invert_rep. pike_subset. simpl. exists pcmid.
+    rewrite END. split; auto. econstructor; eauto.
+  - repeat invert_rep. eapply IHTREE; eauto. pike_subset.
+  - repeat invert_rep. eapply IHTREE; eauto. pike_subset.
+    repeat (econstructor; eauto). pike_subset.
+  - pike_subset.
+  - destruct greedy; inversion CHOICE.
+Qed.
+
+
+Theorem generate_choice:
+  forall tree1 tree2 gm inp code pc b treeactive
+    (TREESTEP: tree_bfs_step (Choice tree1 tree2) gm (idx inp) = StepActive treeactive)
+    (NOSTUTTER: stutters pc code = false)
+    (TT: tree_thread code inp (Choice tree1 tree2, gm) (pc, gm, b)),
+  exists threadactive,
+    epsilon_step rer (pc, gm, b) code inp = EpsActive threadactive /\
+      list_tree_thread code inp treeactive threadactive.
+Proof.
+  intros tree1 tree2 gm inp code pc b treeactive TREESTEP NOSTUTTER TT.
+  unfold tree_bfs_step in TREESTEP. inversion TREESTEP. subst. clear TREESTEP.
+  inversion TT; subst; try no_stutter.
+  remember (Choice tree1 tree2) as TCHOICE.
+  induction TREE; intros; subst; try inversion HeqTCHOICE; subst.
+  - repeat invert_rep. eapply IHTREE; eauto. pike_subset.
+  - repeat invert_rep. exists [(S pc,gm,b);(S end1,gm,b)]. split.
+    + unfold epsilon_step. rewrite FORK. auto.
+    + constructor.
+      * constructor. constructor.
+        apply tt_eq with (actions:=Areg r2::cont); auto.
+        2: { pike_subset. }
+        repeat (econstructor; eauto).
+      * apply tt_eq with (actions:=Areg r1::cont); auto.
+        2: { pike_subset. }
+        eapply cons_bc with (pcmid:=end1).
+        ** constructor; auto.
+        ** eapply jump_bc; eauto.
+  - repeat invert_rep. eapply IHTREE; eauto. pike_subset.
+    repeat (econstructor; eauto). pike_subset.
+  - repeat invert_rep.
+  - (* when the choice comes from a star *)
+    repeat invert_rep. destruct greedy; inversion CHOICE; subst; destruct plus; inversion H1.
+    +                           (* greedy star *)
+      simpl. rewrite FORK. exists [(S pc, gm, b); (S end1, gm, b)]. split; auto.
+      econstructor.
+      * econstructor. constructor.
+        apply tt_eq with (actions:=cont); auto. pike_subset.
+      * apply tt_begin; auto.
+        replace (S (S pc)) with (S pc +1) in RESET by lia.
+        apply tt_reset; auto.
+        apply tt_eq with (actions:=Areg r1 :: Acheck(inp)::Areg(Quantified true 0 +∞ r1)::cont); auto.
+        2: { pike_subset. }
+        apply cons_bc with (pcmid:=end1).
+        { constructor. replace (S pc+1+1) with (S (S (S pc))) by lia. auto. }
+        repeat (econstructor; eauto).
+        replace (S (S pc)) with (S pc + 1) by lia. auto.
+    +                           (* lazy star *)
+      simpl. rewrite FORK. exists [(S end1, gm, b); (S pc, gm, b)]. split; auto.
+      econstructor.
+      * constructor. constructor. apply tt_begin; auto.
+        replace (S (S pc)) with (S pc + 1) in RESET by lia.
+        apply tt_reset; auto.
+        apply tt_eq with (actions:=Areg r1 :: Acheck(inp)::Areg(Quantified false 0 +∞ r1)::cont); auto.
+        2: { pike_subset. }
+        apply cons_bc with (pcmid:=end1).
+        { constructor. replace (S pc+1+1) with (S (S (S pc))) by lia. auto. }
+        repeat (econstructor; eauto).
+        replace (S (S pc)) with (S pc + 1) by lia. auto.
+      * apply tt_eq with (actions:=cont); auto. pike_subset.
+Qed.
+
+
+(* next we combine the generate lemmas together, for the general non-stuttering case *)
+Theorem generate_active:
+  forall tree gm inp code pc b treeactive
+    (TREESTEP: tree_bfs_step tree gm (idx inp) = StepActive treeactive)
+    (NOSTUTTER: stutters pc code = false)
+    (TT: tree_thread code inp (tree, gm) (pc, gm, b)),
+  exists threadactive,
+    epsilon_step rer (pc, gm, b) code inp = EpsActive threadactive /\
+      list_tree_thread code inp treeactive threadactive.
+Proof.
+  intros tree gm inp code pc b treeactive TREESTEP NOSTUTTER TT.
+  destruct tree; simpl in TREESTEP; inversion TREESTEP; subst.
+  - eapply generate_mismatch in TT; auto. exists []. split; eauto. constructor.
+  - eapply generate_choice; eauto.
+  - inversion TT; subst; try no_stutter.
+    eapply subset_semantics in TREE as SUBSETTREE; auto.
+    inversion SUBSETTREE.
+  - eapply generate_checkpass in TT as [nextpc [STEP EQ]]; auto.
+    exists [(nextpc,gm,CanExit)]. split; eauto.
+    constructor; auto. constructor.
+  - inversion TT; subst; try no_stutter.
+    eapply subset_semantics in TREE as SUBSETTREE; auto.
+    inversion SUBSETTREE.
+  - destruct g.
+    + eapply generate_open in TT as [STEP EQ]; auto.
+      exists [(pc+1,GroupMap.open (idx inp) g gm,b)]. split; eauto.
+      constructor; auto. constructor.
+    + eapply generate_close in TT as [STEP EQ]; auto.
+      exists [(pc+1,GroupMap.close (idx inp) g gm,b)]. split; eauto.
+      constructor; auto. constructor.
+    + eapply generate_reset in TT as [STEP EQ]; auto.
+      exists [(pc + 1, GroupMap.reset gl gm, b)]. split; eauto.
+      constructor; auto. constructor.
+  - inversion TT; subst; try no_stutter.
+    eapply subset_semantics in TREE as SUBSETTREE; auto.
+    inversion SUBSETTREE.
+  - inversion TT; subst; try no_stutter.
+    eapply subset_semantics in TREE as SUBSETTREE; auto.
+    inversion SUBSETTREE.
+Qed.
+
+(* TODO: simplify/automate this proof *)
+(* in the case where we are at a stuttering step, we show that we still preserve the invariant *)
+Theorem stutter_step:
+  forall tree gm inp code pc b
+    (TT: tree_thread code inp (tree,gm) (pc,gm,b))
+    (STUTTER: stutters pc code = true),
+  exists nextpc nextb,
+    epsilon_step rer (pc,gm,b) code inp = EpsActive [(nextpc,gm,nextb)] /\
+      tree_thread code inp (tree,gm) (nextpc,gm,nextb).
+Proof.
+  intros tree gm inp code pc b TT STUTTER.
+  inversion TT; subst.
+  (* reset is not stuttering *)
+  2: { unfold stutters in STUTTER. rewrite RESET in STUTTER. inversion STUTTER. }
+  (* at a beginloop instruction *)
+  2: { exists (pc + 1). exists CannotExit. split; try split; auto.
+       simpl. rewrite BEGIN. auto. }
+  (* at a jmp instruction *)
+  generalize dependent pc.
+  induction TREE; intros.
+  - invert_rep. stutter.
+    exists pcstart. exists b. split; try split; try lia.
+    + simpl. rewrite JMP. auto.
+    + apply tt_eq with (actions:=[]); auto; constructor; auto.
+  - invert_rep.
+    { invert_rep. stutter. }
+    exists pcstart. exists CanExit. split; try split; try lia.
+    + simpl. rewrite JMP. auto.
+    + apply tt_eq with (actions:=Acheck strcheck::cont); try constructor; auto; pike_subset.
+  - invert_rep.
+    { invert_rep. stutter. }
+    exists pcstart. exists CannotExit. split; try split; try lia.
+    + simpl. rewrite JMP. auto.
+    + apply tt_eq with (actions:=Acheck strcheck::cont); try constructor; auto; pike_subset.
+  - invert_rep.
+    { invert_rep. stutter. }
+    exists pcstart. exists b. split; try split; try lia.
+    + simpl. rewrite JMP. auto.
+    + apply tt_eq with (actions:=Aclose gid::cont); try constructor; auto; pike_subset.
+  - invert_rep.
+    + invert_rep. invert_rep; try in_subset.
+      eapply IHTREE; eauto. pike_subset.
+    + exists pcstart. exists b. split; try split; try lia.
+      * simpl. rewrite JMP. auto.
+      * apply tt_eq with (actions:=Areg Epsilon :: cont); try constructor; auto; pike_subset.
+  - invert_rep.
+    { invert_rep. invert_rep; try in_subset; try stutter. }
+    exists pcstart. exists b. split; try split; try lia.
+    + simpl. rewrite JMP. auto.
+    + apply tt_eq with (actions:=Areg (Regex.Character cd) :: cont); try constructor; auto; pike_subset.
+      eapply tree_char; eauto.
+  - invert_rep.
+    { invert_rep. invert_rep; try in_subset; try stutter. }
+    exists pcstart. exists b. split; try split; try lia.
+    + simpl. rewrite JMP. auto.
+    + apply tt_eq with (actions:=Areg (Regex.Character cd) :: cont); try constructor; auto; pike_subset.
+  - invert_rep.
+    { invert_rep. invert_rep; try in_subset; try stutter. }
+    exists pcstart. exists b. split; try split; try lia.
+    * simpl. rewrite JMP. auto.
+    * apply tt_eq with (actions:=Areg (Disjunction r1 r2) :: cont); try constructor; auto; pike_subset.
+  - invert_rep.
+    + invert_rep. invert_rep; try in_subset.
+      eapply IHTREE; eauto. pike_subset.
+      repeat (econstructor; eauto).
+    + exists pcstart. exists b. split; try split; try lia.
+      * simpl. rewrite JMP. auto.
+      * apply tt_eq with (actions:=Areg (Sequence r1 r2) :: cont); try constructor; auto; pike_subset.
+  - invert_rep.
+    { invert_rep. invert_rep; try in_subset; try stutter. }
+    exists pcstart. exists b. split; try split; try lia.
+    * simpl. rewrite JMP. auto.
+    * apply tt_eq with (actions:=Areg (Quantified greedy (S min) plus r1) :: cont); try constructor; auto; pike_subset.
+  - pike_subset.
+  - invert_rep.
+    { invert_rep. invert_rep; try in_subset. destruct greedy; stutter. }
+    exists pcstart. exists b. split; try split; try lia.
+    + simpl. rewrite JMP. auto.
+    + destruct plus; [pike_subset|].
+      apply tt_eq with (actions:=Areg (Quantified greedy 0 (NoI.N 1 + +∞)%NoI r1) :: cont); try constructor; auto; pike_subset.
+      eapply tree_quant_free; eauto.
+  - invert_rep.
+    { invert_rep. invert_rep; try in_subset; try stutter. }
+    exists pcstart. exists b. split; try split; try lia.
+    * simpl. rewrite JMP. auto.
+    * apply tt_eq with (actions:=Areg (Group gid r1):: cont); try constructor; auto; pike_subset.
+  - pike_subset.
+  - pike_subset.
+Qed.
+
+
+
+(** * Simulation Invariant  *)
+
+(* This is not, strictly speaking, an inclusion, which explains the second case of this disjunction *)
+(* Sometimes, we add seen pcs on the VM side that do not correspond yet to any seen tree on the tree side *)
+(* this happens during stuttering steps: such pcs are always stuttering, equivalent to the current active tree, *)
+(* but these pcs are not equal to the current pc : they're smaller *)
+(* the relation is then indexed by the current pc *)
+Definition seen_inclusion (c:code) (inp:input) (treeseen:seentrees) (threadseen:seenpcs) (current:option (tree*group_map)) (currentpc:label): Prop :=
+  forall pc b
+    (SEEN: inseenpc threadseen pc b = true),
+  (exists t gm,
+      inseen treeseen t = true /\
+        tree_thread c inp (t, gm) (pc, gm, b))
+  \/
+    (stutters pc c = true /\
+       exists t gm, pc < currentpc /\ current = Some (t,gm) /\
+              tree_thread c inp (t,gm) (pc,gm,b)).
+
+Definition head_pc (threadactive:list thread) : label :=
+  match threadactive with
+  | [] => 0
+  | (pc,_,_)::_ => pc
+  end.
+
+Inductive pike_inv (code:code): pike_tree_state -> pike_vm_state -> Prop :=
+| pikeinv:
+  forall inp treeactive treeblocked threadactive threadblocked best treeseen threadseen
+    (ACTIVE: list_tree_thread code inp treeactive threadactive)
+    (* blocked threads should be equivalent for the next input *)
+    (* nothing to say if there is no next input *)
+    (BLOCKED: forall nextinp, advance_input inp forward = Some nextinp -> list_tree_thread code nextinp treeblocked threadblocked)
+    (* these two properties are needed to ensure the two algorithms stop at he same time *)
+    (ENDVM: advance_input inp forward = None -> threadblocked = [])
+    (ENDTREE: advance_input inp forward = None -> treeblocked = [])
+    (* any pc in threadseen must correspond to a tree in treeseen *)
+    (SEEN: seen_inclusion code inp treeseen threadseen (hd_error treeactive) (head_pc threadactive)),
+    pike_inv code (PTS inp treeactive best treeblocked treeseen) (PVS inp threadactive best threadblocked threadseen)
+| pikeinv_final:
+  forall best,
+    pike_inv code (PTS_final best) (PVS_final best).
+
+
+
+(** * Representation Unicity lemmas  *)
+
+(* tree-thread equivalence can only happen for a single gm *)
+Lemma tt_same_gm:
+  forall t gm1 pc gm2 b code inp,
+    tree_thread code inp (t,gm1) (pc,gm2,b) -> gm1 = gm2.
+Proof.
+  intros t gm1 pc gm2 b code inp H. inversion H; auto.
+Qed.
+
+
+(* A representation cannot start with Reset or BeginLoop *)
+Inductive start_rep: bytecode -> Prop :=
+| start_accept: start_rep Accept
+| start_cons: forall cd, start_rep (Consume cd)
+| start_jmp: forall lbl, start_rep (Jmp lbl)
+| start_fork: forall l1 l2, start_rep (Fork l1 l2)
+| start_open: forall gid, start_rep (SetRegOpen gid)
+| start_close: forall gid, start_rep (SetRegClose gid)
+| start_end: forall lbl, start_rep (EndLoop lbl)
+| start_kill: start_rep KillThread.
+
+Lemma nfa_rep_start:
+  forall r code pc pcend,
+    nfa_rep r code pc pcend ->
+    pc = pcend \/
+      (exists i, get_pc code pc = Some i /\ start_rep i).
+Proof.
+  intros r code pc pcend H. induction H;
+    try solve[left; simpl; auto];
+    try solve[right; eexists; split; eauto; constructor].
+  - destruct IHnfa_rep1 as [SAME1 | [i [START1 REP1]]]; subst.
+    2: { right. eexists. split; eauto. }
+    destruct IHnfa_rep2 as [SAME2 | [i [START2 REP2]]]; subst.
+    + left. auto.
+    + right. eexists. split; eauto.
+  - right. destruct greedy; inversion FORK; eexists; split; eauto; constructor.
+Qed.
+
+Lemma action_rep_start:
+  forall a code pc pcend,
+    action_rep a code pc pcend ->
+    pc = pcend \/
+      (exists i, get_pc code pc = Some i /\ start_rep i).
+Proof.
+  intros a code pc pcend H. destruct a.
+  - inversion H. subst. apply nfa_rep_start in NFA. auto.
+  - inversion H. subst. right. exists (EndLoop pcend). split; auto. constructor.
+  - inversion H. subst. right. exists (SetRegClose g). split; auto. constructor.
+Qed.
+
+Lemma actions_rep_start:
+  forall act code pc i,
+    actions_rep act code pc ->
+    get_pc code pc = Some i ->
+    start_rep i.
+Proof.
+  intros act code pc i H. induction H; intros GET. 
+  - rewrite ACCEPT in GET. inversion GET. constructor.
+  - apply action_rep_start in ACTION as [EQ | [instr [GETSTART START]]].
+    + subst. apply IHactions_rep. auto.
+    + rewrite GETSTART in GET. inversion GET. subst. auto.
+  - rewrite JMP in GET. inversion GET. constructor.
+Qed.
+
+(* rephrasing the lemma below so that induction handles pairs better *)
+Lemma tt_same_interm:
+  forall code inp treegm1 treegm2 thread1 thread2
+    (TT1: tree_thread code inp treegm1 thread1)
+    (TT2: tree_thread code inp treegm2 thread2)
+    (SAMEPC: fst (fst thread1) = fst (fst thread2))
+    (SAMEB: snd thread1 = snd thread2)
+    (SAMEGM1: snd (fst thread1) = snd treegm1)
+    (SAMEGM2: snd (fst thread2) = snd treegm2),
+    fst treegm1 = fst treegm2.
+Proof.
+  intros code inp treegm1 treegm2 thread1 thread2 TT1.
+  generalize dependent thread2. generalize dependent treegm2.
+  induction TT1; intros; subst.
+  - inversion TT2; subst;
+      simpl in SAMEB; simpl in SAMEPC; simpl in SAMEGM1; simpl in SAMEGM2; subst;
+      try solve[eapply actions_rep_start in CONT; eauto; inversion CONT].
+    simpl. subst. symmetry. eapply actions_rep_unicity in CONT; eauto.
+  - inversion TT2; subst;
+      simpl in SAMEB; simpl in SAMEPC; simpl in SAMEGM1; simpl in SAMEGM2; subst;
+      try solve[eapply actions_rep_start in CONT; eauto; inversion CONT].
+    2: { rewrite BEGIN in RESET. inversion RESET. }
+    rewrite RESET in RESET0. inversion RESET0. subst.
+    specialize (IHTT1 _ _ TT (eq_refl _) (eq_refl _) (eq_refl _) (eq_refl _)).
+    simpl in IHTT1. destruct IHTT1. subst. simpl. auto.
+  - inversion TT2; subst;
+      simpl in SAMEB; simpl in SAMEPC; simpl in SAMEGM1; simpl in SAMEGM2; subst;
+      try solve[eapply actions_rep_start in CONT; eauto; inversion CONT].
+    { rewrite BEGIN in RESET. inversion RESET. }
+    specialize (IHTT1 _ _ TT (eq_refl _) (eq_refl _) (eq_refl _) (eq_refl _)).
+    simpl in IHTT1. destruct IHTT1. subst. simpl. auto.
+Qed.
+
+Lemma tt_same_tree:
+  forall code inp t1 gm1 t2 gm2 pc b
+    (TT1: tree_thread code inp (t1,gm1) (pc,gm1,b))
+    (TT2: tree_thread code inp (t2,gm2) (pc,gm2,b)),
+    t1 = t2.
+Proof.
+  intros code inp t1 gm1 t2 gm2 pc b TT1 TT2.
+  eapply tt_same_interm in TT1; eauto. simpl in TT1. auto.
+Qed.
+
+(** * Seen Lemmas *)
+
+
+Lemma initial_inclusion:
+  forall c inp current currentpc,
+    seen_inclusion c inp initial_seentrees initial_seenpcs current currentpc.
+Proof.
+  intros c inp current currentpc. unfold seen_inclusion. intros pc b SEEN.
+  rewrite initial_nothing_pc in SEEN. inversion SEEN.
+Qed.
+
+Lemma add_inclusion:
+  forall treeseen threadseen c inp t pc gm b nextcurrent nextpc
+    (INCL: seen_inclusion c inp treeseen threadseen (Some (t,gm)) pc)
+    (TT: tree_thread c inp (t,gm) (pc,gm,b)),
+    seen_inclusion c inp (add_seentrees treeseen t) (add_thread threadseen (pc, gm, b)) nextcurrent nextpc.
+Proof.
+  intros treeseen threadseen c inp t pc gm b nextcurrent nextpc INCL TT.
+  unfold seen_inclusion in *.
+  intros pc0 b0 SEEN. simpl in SEEN. apply inpc_add in SEEN. destruct SEEN as [EQ|SEEN].
+  - inversion EQ. subst. left. exists t. exists gm. split; auto. apply in_add. left. auto.
+  - specialize (INCL pc0 b0 SEEN).      
+    destruct INCL as [[ts [gms [SEENs TTs]]] | [ST [ts [gms [GEQ [EQ TTS]]]]]].
+    + left. exists ts. exists gms. split; auto. apply in_add. right; auto.
+    + left. exists ts. exists gms. split; auto.
+      apply in_add. left; auto. inversion EQ. auto.
+Qed.
+
+Lemma skip_inclusion:
+  forall code inp treeseen threadseen tree gm currentpc
+    (INCL: seen_inclusion code inp treeseen threadseen (Some (tree, gm)) currentpc)
+    (SEEN: inseen treeseen tree = true),
+  forall current nextpc,
+    seen_inclusion code inp treeseen threadseen current nextpc.
+Proof.
+  intros code inp treeseen threadseen tree gm currentpc INCL SEEN current nextpc.
+  unfold seen_inclusion in *.
+  intros pc b SEENPC.
+  specialize (INCL pc b SEENPC).
+  destruct INCL as [[ts [gms [SEENs TTs]]] | [ST [ts [gms [GEQ [EQ TTS]]]]]].
+  - left. exists ts. exists gms. split; auto.
+  - left. exists ts. exists gms. split; auto. inversion EQ. subst. auto.
+Qed.
+
+Lemma stutter_inclusion:
+  forall code inp treeseen threadseen t gm pc b nextpc
+    (GT: pc < nextpc )
+    (INCL: seen_inclusion code inp treeseen threadseen (Some (t, gm)) pc)
+    (STUTTERS: stutters pc code = true)
+    (TT: tree_thread code inp (t,gm) (pc,gm,b)),
+    seen_inclusion code inp treeseen (add_seenpcs threadseen pc b) (Some (t,gm)) nextpc.
+Proof.
+  intros code inp treeseen threadseen t gm pc b nextpc GT INCL STUTTERS TT.
+  unfold seen_inclusion in *.
+  intros pc0 b0 SEEN.
+  apply inpc_add in SEEN. destruct SEEN as [EQ | SEEN].
+  { inversion EQ. subst. right. split; auto.
+    exists t. exists gm. split; auto. }
+  specialize (INCL pc0 b0 SEEN).
+  destruct INCL as [[ts [gms [SEENs TTs]]] | [ST [ts [gms [GEQ [EQ TTS]]]]]].
+  - left. exists ts. exists gms. split; auto.
+  - right. split; auto. exists ts. exists gms. split; auto. lia.
+Qed.
+
+(** * Code Stuttering Well-formedness *)
+(* to show that a stuttering step cannot lead the PikeVM to immediately memoize something that was not memoized by the PikeTree, we need to show that stutteing instructions always point to a greater pc *)
+
+Definition stutter_wf (code:code) : Prop :=
+  forall pc gm b nextpc nextgm nextb inp,
+    stutters pc code = true ->
+    epsilon_step rer (pc,gm,b) code inp = EpsActive[(nextpc,nextgm,nextb)] ->
+    pc < nextpc.
+
+Lemma nth_nil:
+  forall (A:Type) i, @nth_error A [] i = None.
+Proof.
+  intros A i. destruct i; simpl; auto.
+Qed.
+
+Lemma nfa_rep_incr:
+  forall r code start endl,
+    nfa_rep r code start endl ->
+    start <= endl.
+Proof.
+  intros r code start endl H. induction H; try lia.
+Qed.
+
+(* every jump in the code jumps to a strictly bigger label *)
+(* this will help prevent loops of stuttering steps in the PikeVM *)
+Lemma compile_jumps:
+  forall r code start endl pc next,
+    nfa_rep r code start endl ->
+    pc >= start ->
+    pc < endl ->
+    get_pc code pc = Some (Jmp next) ->
+    pc < next.
+Proof.
+  intros r code start endl pc next REP GE LT GET.
+  generalize dependent pc. induction REP; intros.
+  - lia.
+  - assert (pc = lbl) by lia. subst.
+    rewrite CONSUME in GET. inversion GET.
+  - apply nfa_rep_incr in REP1 as INCR1.
+    apply nfa_rep_incr in REP2 as INCR2.
+    assert (pc = start \/ pc >= S start) as [ST|H] by lia.
+    (* Fork *)
+    { subst. rewrite FORK in GET. inversion GET. }
+    assert (pc < end1 \/ pc >= end1) as [R1|H1] by lia.
+    (* in r1 *)
+    { apply IHREP1; auto. }
+    assert (pc = end1 \/ pc >= S end1) as [J|H2] by lia.
+    (* the jmp *)
+    { subst. rewrite JMP in GET. inversion GET. lia. }
+    (* in r2 *)
+    apply IHREP2; auto.
+  - apply nfa_rep_incr in REP1 as INCR1.
+    apply nfa_rep_incr in REP2 as INCR2.
+    assert (pc < end1 \/ pc >= end1) as [H1|H2] by lia.
+    (* in r1 *)
+    { apply IHREP1; auto. }
+    (* in r2 *)
+    apply IHREP2; auto.
+  - apply nfa_rep_incr in REP as INC.
+    assert (pc = start \/ pc >= S start) as [FOR|H] by lia.
+    (* fork *)
+    { subst. rewrite FORK in GET. destruct greedy; inversion GET. }
+    assert (pc = S start \/ pc >= S (S start)) as [BEG|H1] by lia.
+    (* Begin *)
+    { subst. rewrite BEGIN in GET. inversion GET. }
+    assert (pc = S (S start) \/ pc >= S (S (S start))) as [RES|H2] by lia.
+    (* Reset *)
+    { subst. rewrite RESET in GET. inversion GET. }
+    assert (pc < end1 \/ pc = end1) as [R1|H3] by lia.
+    (* in r1 *)
+    { apply IHREP; auto. }
+    (* endloop *)
+    subst. rewrite END in GET. inversion GET.
+  - apply nfa_rep_incr in REP as INC.
+    assert (pc = start \/ pc >= S start) as [ST|H] by lia.
+    (* open *)
+    { subst. rewrite OPEN in GET. inversion GET. }
+    assert (pc = end1 \/ pc < end1) as [END|H1] by lia.
+    (* close *)
+    { subst. rewrite CLOSE in GET. inversion GET. }
+    (* in r1 *)
+    apply IHREP; auto.
+  - assert (pc = lbl) by lia. subst.
+    rewrite KILL in GET. inversion GET.
+Qed.
+
+
+(* every compiled code is well-formed *)
+Lemma compile_stutter_wf:
+  forall r code fresh,
+    compile r 0 = (code, fresh) ->
+    stutter_wf code.
+Proof.
+  intros r code fresh H.
+  eapply compile_nfa_rep with (prev:=[]) in H as REP; simpl; auto.
+  simpl in REP. apply fresh_correct in H. simpl in H. subst.
+  unfold stutter_wf. unfold stutters. unfold get_pc.
+  intros pc gm b nextpc nextgm nextb inp H H0.
+  destruct (nth_error code pc) eqn:NTH.
+  2: { inversion H. }
+  destruct b0; inversion H; simpl in H0; unfold get_pc in H0; rewrite NTH in H0;
+    inversion H0; subst; try lia.
+  eapply compile_jumps; eauto; try lia.
+  apply nth_error_Some. rewrite NTH. intros HI. inversion HI.
+Qed.
+
+Theorem compilation_stutter_wf:
+  forall r code,
+    compilation r = code ->
+    stutter_wf code.
+Proof.
+  unfold compilation. intros r code H.
+  destruct (compile r 0) as [r_code fresh] eqn:COMP. subst.
+  apply compile_stutter_wf in COMP.
+  unfold stutter_wf, stutters, get_pc.
+  intros pc gm b nextpc nextgm nextb inp H H0.
+  destruct (nth_error (r_code ++ [Accept]) pc) eqn:NTH.
+  2: { inversion H. }
+  assert (HL: pc < length (r_code ++ [Accept])).
+  { eapply nth_error_Some. rewrite NTH. intros HI. inversion HI. }
+  rewrite app_length in HL. simpl in HL.
+  assert (pc = length (r_code) \/ pc < length (r_code)) as [ACC|H1] by lia.
+  (* accept *)
+  { subst. assert (get_pc (r_code ++ [Accept]) (length r_code) = get_pc [Accept] 0).
+    - apply get_first.
+    - unfold get_pc in H1. simpl in H1. rewrite H1 in NTH. inversion NTH. subst.
+      inversion H. }
+  (* inside the code *)
+  assert (get_pc r_code pc = Some b0).
+  { rewrite nth_error_app1 in NTH; auto. }
+  unfold stutter_wf in COMP.
+  assert (epsilon_step rer (pc,gm,b) r_code inp = EpsActive [(nextpc,nextgm,nextb)]).
+  { simpl in H0. unfold get_pc in H0. rewrite NTH in H0.
+    simpl. rewrite H2.
+    destruct b0; auto. }
+  eapply COMP; eauto.
+  unfold stutters. rewrite H2. destruct b0; auto.
+Qed.
+
+  
+
+
+(** * Invariant Initialization  *)
+
+(* the initial states of both smallstep semantics are related with the invariant *)
+Lemma initial_pike_inv:
+  forall r inp tree code
+    (TREE: bool_tree rer [Areg r] inp CanExit tree)
+    (COMPILE: compilation r = code)
+    (SUBSET: pike_regex r),
+    pike_inv code (pike_tree_initial_state tree inp) (pike_vm_initial_state inp).
+Proof.
+  intros r inp tree code TREE COMPILE SUBSET.
+  unfold compilation in COMPILE. destruct (compile r 0) as [c fresh] eqn:COMP.
+  apply compile_nfa_rep with (prev := []) in COMP as REP; auto. simpl in REP.
+  apply fresh_correct in COMP. simpl in COMP. subst.
+  eapply pikeinv; auto.
+  - econstructor.
+    + constructor.
+    + apply tt_eq with (actions:=[Areg r]); auto.
+      2: { pike_subset. }
+      eapply cons_bc; constructor.
+      * apply nfa_rep_extend; eauto.
+      * replace (length c) with (length c + 0) by auto.
+        rewrite get_prefix. auto.
+  - constructor.
+  - apply initial_inclusion.
+Qed.
+
+(** * Invariant Preservation  *)
+
+(* identifying states of the VM that are going to take a skip step *)
+Definition skip_state (pvs:pike_vm_state) : bool :=
+  match pvs with
+  | PVS_final _ => false
+  | PVS inp active best blocked seen =>
+      match active with
+      | [] => false
+      | (pc,gm,b)::active => inseenpc seen pc b
+      end
+  end.
+  
+
+Theorem invariant_preservation:
+  forall code pts1 pvs1 pvs2
+    (STWF: stutter_wf code)
+    (INV: pike_inv code pts1 pvs1)
+    (VMSTEP: pike_vm_step rer code pvs1 pvs2),
+    (* either we make a step on both sides, preserving invariant *)
+    (
+      exists pts2,
+        pike_tree_step pts1 pts2 /\
+          pike_inv code pts2 pvs2
+    )
+    \/
+      (* or we make a stuttering step, preserving invariant with pts1 *)
+      (
+          pike_inv code pts1 pvs2
+      ).
+Proof.
+  intros code pts1 pvs1 pvs2 STWF INV VMSTEP.
+  inversion INV; subst.
+  (* Final states make no step *)
+  2: { inversion VMSTEP. }
+  destruct (skip_state (PVS inp threadactive best threadblocked threadseen)) eqn:SKIP.
+  (* skip states are performed in lockstep *)
+  { left. destruct threadactive as [|[[pc gm] b] active]; simpl in SKIP.
+    { inversion SKIP. }
+    destruct treeactive as [|[tree gmt] treeactive]; inversion ACTIVE; subst.
+    inversion VMSTEP; subst; try simpl in UNSEEN;
+      try rewrite UNSEEN in SKIP; inversion SKIP.    
+    apply SEEN in SKIP as [[teq [gmeq [SEENEQ TTEQ]]] | [STUTTER [t' [gm' [GEQ [EQ TTS]]]]]].
+    - assert (teq = tree).
+      { eapply tt_same_tree; eauto. }
+      subst.
+      exists (PTS inp treeactive best treeblocked treeseen).
+      split.
+      + apply ptss_skip; auto.
+      + eapply pikeinv; eauto.
+        simpl in SEEN. eapply skip_inclusion; eauto.
+    - simpl in GEQ. lia.
+  }
+  destruct treeactive as [|[t gm] treeactive].
+  {
+    (* no more active trees or threads *)
+    inversion ACTIVE; subst.
+    destruct treeblocked as [|[tblocked gmblocked] treeblocked].
+    (* final step *)
+    - assert (pvs2 = (PVS_final best)).
+      { eapply pikevm_deterministic; eauto.
+        destruct (advance_input inp) eqn:ADV; try solve[constructor; auto].
+        specialize (BLOCKED i (eq_refl (Some i))). inversion BLOCKED; subst. constructor. }
+      subst. left. exists (PTS_final best). split; constructor.
+    (* nextchar *)
+    - destruct (advance_input inp) eqn:ADV.
+      2: { specialize (ENDTREE (eq_refl None)). inversion ENDTREE. }
+      specialize (BLOCKED i (eq_refl (Some i))). inversion BLOCKED; subst.
+      assert (pvs2 = PVS i ((pc,gmblocked,b)::threadlist) best [] initial_seenpcs).
+      { eapply pikevm_deterministic; eauto. constructor. auto. }
+      subst. left. exists (PTS i ((tblocked,gmblocked)::treeblocked) best [] initial_seentrees).
+      apply advance_next in ADV. subst.
+      split; try econstructor; eauto.
+      + intros nextinp H. constructor.
+      + apply initial_inclusion.
+  }
+  (* there is an active tree/thread *)
+  destruct threadactive as [|[[pc gm'] b] threadactive]; inversion ACTIVE; subst.
+  rename gm' into gm.
+  destruct (stutters pc code) eqn:STUTTERS.
+  {
+    (* stuttering step *)
+    right. apply stutter_step in TT as H; auto.
+    destruct H as [nextpc [nextb [EPSSTEP TT2]]]; subst.
+    assert (pvs2 = (PVS inp ([(nextpc, gm, nextb)] ++ threadactive) best threadblocked (add_thread threadseen (pc,gm,b)))).
+    { eapply pikevm_deterministic; eauto. eapply pvss_active; eauto. }
+    subst; simpl; auto. eapply pikeinv; simpl; eauto.
+    - constructor; eauto.
+    - (* Here we use that the code is stutter-well-formed *)
+      simpl in SEEN. eapply stutter_inclusion; eauto.
+  }
+  destruct (tree_bfs_step t gm (idx inp)) eqn:TREESTEP.
+  (* active *)
+  - left. eapply generate_active in TREESTEP as H; eauto. destruct H as [newthreads [EPS LTT2]].
+    assert (pvs2 = PVS inp (newthreads ++ threadactive) best threadblocked (add_thread threadseen (pc,gm,b))).
+    { eapply pikevm_deterministic; eauto. constructor; auto. }
+    subst. exists (PTS inp (l ++ treeactive) best treeblocked (add_seentrees treeseen t)). split.
+    + eapply ptss_active; eauto.
+    + eapply pikeinv; try (eapply add_inclusion; eauto); try constructor; eauto.
+      apply ltt_app; eauto.
+  (* match *)
+  - left. eapply generate_match in TREESTEP as THREADSTEP; eauto.
+    assert (pvs2 = PVS inp [] (Some (inp,gm_of (pc,gm,b))) threadblocked (add_thread threadseen (pc,gm,b))).
+    { eapply pikevm_deterministic; eauto. constructor; auto. }
+    subst. exists (PTS inp [] (Some (inp,gm)) treeblocked (add_seentrees treeseen t)). split.
+    + constructor; auto.
+    + eapply pikeinv; try (eapply add_inclusion; eauto); try constructor; eauto.
+  (* blocked *)
+  - left. specialize (generate_blocked _ _ _ _ _ _ _ TREESTEP STUTTERS TT) as [EPS2 [TT2 [nexti ADVANCE]]].
+    assert (pvs2 = PVS inp threadactive best (threadblocked ++ [(pc+1,gm,CanExit)]) (add_thread threadseen (pc,gm,b))).
+    { eapply pikevm_deterministic; eauto. constructor; auto. }
+    subst. exists (PTS inp treeactive best (treeblocked ++ [(t0,gm)]) (add_seentrees treeseen t)). split.
+    + eapply ptss_blocked; eauto.
+    + eapply pikeinv; try (eapply add_inclusion; eauto); try constructor; eauto.
+      2: { intros H. rewrite ADVANCE in H. inversion H. }
+      2: { intros H. rewrite ADVANCE in H. inversion H. }
+      intros nextinp H. specialize (BLOCKED nextinp H).
+      apply ltt_app; eauto. specialize (TT2 nextinp H).
+      eapply ltt_cons. constructor. auto.
+Qed.
+
+End PikeEquiv.
